\subsection{Definition of Abstract Map}
For any concrete map $\CMap$,
if abstract key $\AKey$ and abstract value $\AVal$ is defined,
and there exists a sound relation $\wsf{isRelated}$ 
that abstracts \emph{may equal} of two abstract key valaues,
we can define a abstract map $\AMap$.\\

$\begin{array}{l}
\poset(\CMap) \xrightarrow{\alpha_{m}}
\AMap \xrightarrow{\gamma_{m}} \poset(\CMap) \vspace{1mm} \\
\poset(\CKey) \xrightarrow{\alpha_{k}} 
\AKey \xrightarrow{\gamma_{k}} \poset(\CKey) \\
\poset(\CVal) \xrightarrow{\alpha_{v}} 
\AVal \xrightarrow{\gamma_{v}} \poset(\CVal) \vspace{1mm} \\
\wsf{isRelated} \in \AKey \times \AKey \rightarrow \textbf{Boolean} \\
\end{array}$\\\\
Formal definition of $\alpha_m$ and $\gamma_m$ are at section \ref{sec:galois}.\\
Our definition of abstract map consist of 2 parts:
\begin{enumerate}
\item $\Map$ part which is a partial map from $\AKey$ to $\AVal$, and
\item $\Defset$ part which is a set of definitely existing key values.
The size of $\Defset$ may be infinite, 
for example, bottom of $\AMap$ has the whole $\CKey$ as its $\Defset$.
\end{enumerate}
$\begin{array}{l}
\hat{m},\ \langle \emph{map},\ \emph{defset} \rangle
\in \AMap = (\AKey \rightarrowtail \AVal)
\times \poset(\CKey)\\
\quad \Map(\langle \emph{map},\ \emph{defset} \rangle) = 
\emph{map} \in \AKey \rightarrowtail \AVal \\
\quad \Defset(\langle \emph{map},\ \emph{defset} \rangle) = 
\emph{defset} \in \poset(\CKey) \\
\quad \Dom(\langle \emph{map},\ \emph{defset} \rangle) = 
\{ \hat{k} \mid \emph{map} 
\textrm{ has a mapped value for key } \hat{k} \} \in \poset(\AKey) \\
\end{array}$

\subsubsection{Partial Order and Join}
$\begin{array}{rl}
\hat{m}_1 \po_m \hat{m}_2 = & 
\forall \hat{k}_1 \in \Dom(\hat{m}_1) \cdot 
\exists \hat{k}_2 \in \Dom(\hat{m}_2) :
\hat{k}_1 \po_k \hat{k}_2
\land \Map(\hat{m}_1)(\hat{k}_1) \po_v \Map(\hat{m}_2)(\hat{k}_2) \\
& \land\ \Defset(\hat{m}_2) \subseteq \Defset(\hat{m}_1) \\
\end{array}$\\\\
$\begin{array}{l}
\hat{m}_1 \sqcup_m \hat{m}_2 =
\langle \emph{map}_1 \cup \emph{map}_2 \cup \emph{map}_{\cap},\
\Defset(\hat{m}_1) \cap \Defset(\hat{m}_2) \rangle \\
\quad \begin{array}{rl} \textrm{where} 
& \emph{map}_1 = \left \{~ [ \hat{k} \mapsto \Map(\hat{m}_1)(\hat{k}) ] ~\mid~
\hat{k} \in \Dom(\hat{m}_1) 
\setminus \Dom(\hat{m}_2) ~\right \} \\
& \emph{map}_2 = \left \{~ [ \hat{k} \mapsto \Map(\hat{m}_2)(\hat{k}) ] ~\mid~
\hat{k} \in \Dom(\hat{m}_2)
\setminus \Dom(\hat{m}_1) ~\right \} \\
& \emph{map}_{\cap} = \left \{~ [ \hat{k} \mapsto 
\Map(\hat{m}_1)(\hat{k}) \sqcup_v \Map(\hat{m}_2)(\hat{k}) ] ~\mid~
\hat{k} \in \Dom(\hat{m}_1) 
\cap \Dom(\hat{m}_2) ~\right \} \\
\end{array} \\
\end{array}$

\subsubsection{Abstraction and Concretization} \label{sec:galois}
The abstract map $\AMap$ has Golois connection with concrete map $\CMap$.
\begin{center}
\textbf{Theorem }
$\forall \emph{mset} \in \poset(\CMap), ~ 
\forall \hat{m} \in \AMap, ~
\alpha_m(\emph{mset}) \po_m \hat{m}
\Longleftrightarrow
\emph{mset} \subseteq \gamma_m(\hat{m})$
\end{center}
$\gamma_m$ and $\alpha_m$ are defined as follow: \\

$\begin{array}{l}
\forall \emph{mset} \in \poset(\CMap) \cdot \\ 
\left \{
\begin{array}{l}
\alpha_m(\varnothing) = \bot_m \\
\quad \textrm{where } \bot_m = \langle \varnothing,\ \textbf{String} \rangle \\
\alpha_m(\emph{mset}) =
\langle \emph{map},\ \bigcap \left \{ \Dom(m) \mid m \in \emph{mset} \right \} \rangle \\
\quad \begin{array}{ll}\textrm{where} 
& \emph{map} = \left \{
[ \hat{k} \mapsto \alpha_{v}( \{ m(k') \mid m \in \emph{mset} 
\land k' \in \Dom(m) \land \alpha_k(\{k'\}) = \hat{k} \} ) ]
\mid \hat{k} \in \emph{S}  \right \} \\
& \emph{S} = \left \{ 
\alpha_k(\{k\}) \mid m \in \emph{mset} \land k \in \Dom(m) \right \}\\
\end{array}\\
\end{array} \right. \\\\

\forall \hat{m} \in \AMap \cdot \\
\quad \gamma_{m}(\hat{m}) = \bigcup \left \{ \emph{mset} ~\mid~
\alpha_{m}(\emph{mset}) \po_m \hat{m} \right \} \\
\end{array}$\\\\\\
\textbf{Monotonicity of $\alpha_m$}
\begin{center}
$\forall \emph{mset}_1, \emph{mset}_2 \in \poset(\CMap), ~
\emph{mset}_1 \subseteq \emph{mset}_2
\Rightarrow
\alpha_m(\emph{mset}_1) \po_m \alpha_m(\emph{mset}_2)$
\end{center}
\textbf{Proof } 
$\forall \emph{mset}_1, \emph{mset}_2 \in \poset{\CMap},~ 
\emph{mset}_1 \subseteq \emph{mset}_2, ~$
\begin{itemize}
\item \textbf{If} $\emph{mset}_1 = \varnothing$,
since $\alpha_m(\emph{mset}_1) = \bot_m$,
$\alpha_m(\emph{mset}_1) \po_m \alpha_m(\emph{mese}_2)$.
\item \textbf{If} $\emph{mset}_2 = \varnothing$,
$\emph{mset}_1$ must be $\varnothing$ by $\emph{mset}_1 \subseteq \emph{mset}_2$.
Then $\alpha_m(\emph{mset}_1) = \bot_m \po_m \alpha_m(\emph{mset}_2)$.
\item\textbf{If} $\emph{mset}_1 \neq \varnothing$, and $\emph{mset}_2 \neq \varnothing$, \\
By definition of $\alpha_m$ and $\po_m$, we need to prove that
\begin{enumerate}[label=({\arabic*})]
\item $\forall \hat{k}_1 \in \emph{S}_1 \cdot \exists \hat{k}_2 \in \emph{S}_2:
\hat{k}_1 \po_k \hat{k}_2 \land \emph{map}_1(\hat{k}_1) \po_v \emph{map}_2(\hat{k}_2) ~ $
where \\
$\begin{array}{l}
\quad \emph{map}_1 = \left \{[ \hat{k}_1 \mapsto \alpha_{v}( \{ m_1(k_1') \mid m_1 \in \emph{mset}_1
\land k_1' \in \Dom(m_1) \land \alpha_k(\{k_1'\}) = \hat{k}_1 \} ) ]
\mid \hat{k}_1 \in \emph{S}_1  \right \}\\
\land~ \emph{map}_2 = \left \{[ \hat{k}_2 \mapsto \alpha_{v}( \{ m_2(k_2') \mid m_2 \in \emph{mset}_2
\land k_2' \in \Dom(m_2) \land \alpha_k(\{k_2'\}) = \hat{k}_2 \} ) ]
\mid \hat{k}_2 \in \emph{S}_2  \right \}\\
\land~ \emph{S}_1 = \{ \alpha_k(\{ k_1 \}) \mid m_1 \in \emph{mset}_1 \land k_1 \in \Dom(m_1) \} \\
\land~ \emph{S}_2 = \{ \alpha_k(\{ k_2 \}) \mid m_2 \in \emph{mset}_2 \land k_2 \in \Dom(m_2) \} \\
\end{array}$
\item $\bigcap\{ \Dom(m_2) \mid m_2 \in \emph{mset}_2\} \subseteq 
\bigcap\{ \Dom(m_1) \mid m_1 \in \emph{mset}_1\}$
\end{enumerate}
Prove (1). 
\begin{enumerate}[label={\arabic*})]
\item For arbitrary $\hat{k} \in \AKey$, $\alpha_v(\emph{vset}_1) \po_v \alpha_v(\emph{vset}_2)$ where \\
$\begin{array}{l}
\quad \emph{vset}_1 = \{m_1(k_1') \mid 
m_1 \in \emph{mset}_1 \land k_1' \in \Dom(m_1) \land \alpha_k(\{k_1'\}) = \hat{k} \} \\
\land ~ \emph{vset}_2 = \{m_2(k_2') \mid 
m_2 \in \emph{mset}_2 \land k_2' \in \Dom(m_2) \land \alpha_k(\{k_2'\}) = \hat{k} \} \\
\end{array}$\\
If there is no $k_1' \in \Dom(m_1) \land m_1 \in \emph{mset}_1$ such that $\alpha_k(\{k_1'\}) = \hat{k}$,
then $\emph{vset}_1 = \varnothing \subseteq \emph{vset}_2$.\\
If $m_1 \in \emph{mset}_1$ then $m_1 \in \emph{mset}_2$ as $\emph{mset}_1 \subseteq \emph{mset}_2$.
Therefore if there exists $k_1' \in \Dom(m_1) \land m_1 \in \emph{mset}_1$ 
such that $\alpha_k(\{k_1'\}) = \hat{k}$,
then $\emph{vset}_1 \subseteq \emph{vset}_2$.\\
By monotonicity of $\alpha_v$, $\alpha_v(\emph{vset}_1) \po_v \alpha_v(\emph{vset}_2)$.
\item $\{ \alpha_k(\{ k_1 \}) \mid m_1 \in \emph{mset}_1 \land k_1 \in \Dom(m_1) \}
\subseteq \{ \alpha_k(\{ k_2 \}) \mid m_2 \in \emph{mset}_2 \land k_2 \in \Dom(m_2) \}$ \\
as $\emph{mset}_1 \subseteq \emph{mset}_2$.
\end{enumerate}
By 1) and 2), $\forall \hat{k} \in \emph{S}_1, 
\exists \hat{k} \in \emph{S}_2: \hat{k} \po_k \hat{k}
\land \emph{map}_1(\hat{k}) \po_v \emph{map}_2(\hat{k})$ \vspace{1mm}\\
Prove (2). It is obvious since $\emph{mset}_1 \subseteq \emph{mset}_2$. \vspace{1mm}\\
Thus $\alpha_m(\emph{mset}_1) \po_m \alpha_m(\emph{mset}_2)$.
\end{itemize}
\textbf{Join morphism of $\alpha_m$}
\begin{center}
$\forall \emph{msetset} \in \poset(\poset(\CMap)), ~
\alpha_m(\bigcup\emph{msetset})
=\bigsqcup_m\{ \alpha_m(\emph{mset}) \mid \emph{mset} \in \emph{msetset}\}$
\end{center}
\textbf{Proof } $\forall \emph{msetset} \in \poset(\poset(\CMap))$
\begin{itemize}
\item \textbf{If } $\bigcup \emph{msetset} = \varnothing$, 
Then
\begin{enumerate}[label={\arabic*)}]
\item $\alpha_m(\bigcup \emph{msetset}) = \bot_m$.
\item $\forall \emph{mset} \in \emph{msetset},~ \emph{mset} = \varnothing$.\\
Thus $\bigsqcup_m\{\alpha_m(\emph{mset}) \mid \emph{mset} \in \emph{msetset}\}
= \bigsqcup_m \{ \bot_m \mid \emph{mset} \in \emph{msetset} \}
= \bot_m$.
\end{enumerate}
Therefore, 
$\alpha_m(\bigcup \emph{msetset}) = \bot_m
= \bigsqcup_m\{\alpha_m(\emph{mset}) \mid \emph{mset} \in \emph{msetset}\} $.
\item \textbf{If }
$\bigcup\emph{msetset} \neq \varnothing$, 
let $\hat{m}_l = \alpha_m(\bigcup \emph{msetset})$
and $\hat{m}_r = \bigsqcup_m\{ \alpha_m(\emph{mset}) \mid \emph{mset} \in \emph{msetset} \}$.
Then we need to prove $\Map(\hat{m}_l) = \Map(\hat{m}_r) 
\land \Defset(\hat{m}_l) = \Defset(\hat{m}_r)$. \vspace{1mm} \\
Prove $\Map(\hat{m}_l) = \Map(\hat{m}_r)$.
\begin{enumerate}[label={\arabic*)}]
\item $\Dom(\hat{m}_l) = \Dom(\hat{m}_r)$. \vspace{1mm} \\
$\Dom(\hat{m}_l) = \{ \alpha_k(\{k\}) \mid m \in \bigcup\emph{msetset} \land k \in \Dom(m) \}$
by definition of $\alpha_m$.\\
For arbitrary $\hat{m}_1, \hat{m}_2 \in \AMap$, 
$\Dom(\hat{m}_1 \sqcup_m \hat{m}_2) = \Dom(\hat{m}_1) \cup \Dom(\hat{m}_2)$
by definition of $\sqcup_m$.
Thus $\Dom(\hat{m}_r) = \bigcup \{ \Dom(\alpha_m(\emph{mset})) \mid \emph{mset} \in \emph{msetset} \}$, and \\ 
$\Dom(\hat{m}_r ) = \{ \alpha_k(\{k\}) 
\mid k \in \Dom(m) \land m \in \emph{mset} \land \emph{mset} \in \emph{msetset} \}$
by definition of $\alpha_m$. \vspace{1mm} \\
Therefore $\Dom(\hat{m}_l) = \Dom(\hat{m}_r)$.
\item $\forall \hat{k} \in \Dom(\hat{m}_l) \cdot \Map(\hat{m}_l)(\hat{k}) = \Map(\hat{m}_r)(\hat{k})$.\\
$\begin{array}{ll}
& \Map(\hat{m}_l)(\hat{k}) \\
= & \alpha_v(\{ m(k') \mid m \in \bigcup \emph{msetset} \land k' \in \Dom(m) \land \alpha_k(\{k'\}) = \hat{k} \})
\textrm{ by definition of } \alpha_m.\\
= & \bigsqcup_v\{ \alpha_v(\{ m(k') \mid m \in \emph{mset} \land k' \in \Dom(m) \land \alpha_k(\{k'\}) = \hat{k} \})
\mid \emph{mset} \in \emph{msetset} \} \\
& \textrm{ by Join morphism of } \alpha_v.\\
\end{array}$ \vspace{1mm} \\
$\forall \hat{k} \in \Dom(\hat{m}_l) \cdot \hat{k} \in \Dom(\hat{m}_r)$ by 1). \vspace{1mm}\\
$\begin{array}{ll}
& \Map(\hat{m}_r)(\hat{k}) \\
= & \bigsqcup_v\{ \Map(\hat{m})(\hat{k}') 
\mid \hat{k}' = \hat{k} \land \hat{k}' \in \Dom(\hat{m}) 
\land \hat{m} = \alpha_m(\emph{mset}) \land \emph{mset} \in \emph{msetset} \} \\
& \textrm{ by definition of } \sqcup_m.\\
= & \bigsqcup_v \left \{ \emph{map}(\hat{k})
\middle| \begin{array}{l} 
\emph{map} = \left \{ \left[ \hat{k} \mapsto \alpha_v \left(
\left \{ m(k') \middle| \begin{array}{l} 
m \in \emph{mset}\\
\land k' \in \Dom(m)\\
\land \alpha_k(\{k'\}) = \hat{k}\end{array} \right \}
\right) \right] \middle| \hat{k} \in \emph{S} \right \} \\
~ \land \hat{k}' = \hat{k} \land \hat{k}' \in \emph{S} \\
~ \land \emph{S} = \{ \alpha_k(\{k\}) \mid k \in \Dom(m) \land m \in \emph{mset} \}
\land \emph{mset} \in \emph{msetset}\\
\end{array} \right \} \\
& \textrm{ by definition of } \alpha_m.\\
= & \bigsqcup_v \{ \alpha_v(\{ m(k') \mid k' \in \Dom(m) \land \alpha_k(\{ k' \}) = \hat{k} 
\land m \in \emph{mset} \}) \mid \emph{mset} \in \emph{msetset}\}\\
\end{array}$ \vspace{1mm}\\
Therefore $\forall \hat{k} \in \Dom(\hat{m}_l) = \Dom(\hat{m}_r) \cdot 
\Map(\hat{m}_l)(\hat{k}) = \Map(\hat{m}_r)(\hat{k})$.
\end{enumerate}
By 1) and 2), $\Map(\hat{m}_l) = \Map(\hat{m}_r)$. \vspace{2mm} \\
Prove $\Defset(\hat{m}_l) = \Defset(\hat{m}_r)$. \vspace{1mm} \\
$\Defset(\hat{m}_l) = \bigcap \left \{ \Dom(m) \mid m \in 
\bigcup \emph{msetset} \right \}$ and \\
$\Defset(\hat{m}_r) = \bigcap \left \{ \bigcap \{ \Dom(m) \mid m \in \emph{mset} \} \mid
\emph{mset} \in \emph{msetset} \right \}$ by definition of $\alpha_m$ and $\sqcup_m$. \vspace{1mm} \\
We can simply write it again as follow: \vspace{1mm} \\
$\bigcap \left \{ \Dom(m) \mid m \in \bigcup \emph{msetset} \right \} \\
= \bigcap \{ \Dom(m) \mid m \in \emph{mset} \land \emph{mset} \in \emph{msetset} \} \\
= \bigcap \left \{ \bigcap \{ \Dom(m) \mid m \in \emph{mset} \} \mid \emph{mset} \in \emph{msetset} \right \}$
\vspace{1mm} \\
Thus $\Defset(\hat{m}_l) = \Defset(\hat{m}_r)$. \vspace{1mm} \\
To sum up, $\hat{m}_l = \hat{m}_r$. $i.e.$, 
$\alpha_m(\bigcup \emph{msetset} )
=\bigsqcup_m\{ \alpha_m(\emph{mset}) \mid \emph{mset} \in \emph{msetset}\}$.
\end{itemize}
\textbf{Proof of Theorem }
$\forall \emph{mset} \in \poset(\CMap), ~ 
\forall \hat{m} \in \AMap, ~$
\begin{enumerate}[label={(\arabic*)}]
\item
$\alpha_m(\emph{mset}) \po_m \hat{m}
\Rightarrow
\emph{mset} \subseteq \gamma_m(\hat{m})$ \\
It is obvious by the definition of $\gamma_m$. \hfill $\square$
\item
$\emph{mset} \subseteq \gamma_m(\hat{m})
\Rightarrow
\alpha_m(\emph{mset}) \po_m \hat{m}$ \\
$\emph{mset} \subseteq \gamma_m(\hat{m})
\Rightarrow \alpha_m(\emph{mset}) \po_m \alpha_m(\gamma_m(\hat{m}))$
by \textbf{Monotonicity of $\alpha_m$}.\\
$\alpha_m(\gamma_m(\hat{m})) = 
\alpha_m(\bigcup\{ \emph{mset}' \mid \alpha_m(\emph{mset}') \po_m \hat{m}\}) = 
\bigsqcup_m\{\alpha_m(\emph{mset}') \mid \alpha_m(\emph{mset}') \po_m \hat{m} \}$
by the definition of $\gamma_m$ and \textbf{Join morphism of $\alpha_m$}. \\
$\bigsqcup_m\{\alpha_m(\emph{mset}') \mid \alpha_m(\emph{mset}') \po_m \hat{m} \}
\po_m \hat{m}$, therefore $\alpha_m(\emph{mset}) \po_m \hat{m}$. \hfill $\square$
\end{enumerate}
